Test/NonDetState.lean
@@ -1,0 +1,43 @@
+import Veil
+
+veil module NonDetStateTest
+
+type address
+
+relation initial_msg (originator : address) (dst : address) (r : address) (v : address)
+individual x : Bool
+
+#gen_state
+
+after_init {
+  initial_msg O D R V := False
+  x := False
+}
+
+action nondet = {
+  let st' ← pick σ
+  set st'
+}
+
+action noop (n : address) = {
+  pure ()
+}
+invariant True
+
+#gen_spec
+
+/--
+info: Initialization must establish the invariant:
+  inv_0 ... ✅
+The following set of actions must preserve the invariant and successfully terminate:
+  nondet
+    termination ... ✅
+    inv_0 ... ✅
+  noop
+    termination ... ✅
+    inv_0 ... ✅
+-/
+#guard_msgs in
+#check_invariants
+
+end NonDetStateTest
